Add motives for J and if

beta/join.v
@@ -84,17 +84,18 @@ Inductive Par : tm -> tm -> Prop :=
   (A0 ⇒ A1) ->
   (* ---------- *)
   (tEq a0 b0 A0) ⇒ (tEq a1 b1 A1)
-| P_J t0 a0 b0 p0 t1 a1 b1 p1 :
+| P_J A0 A1 t0 a0 b0 p0 t1 a1 b1 p1 :
+  (A0 ⇒ A1) ->
   (t0 ⇒ t1) ->
   (a0 ⇒ a1) ->
   (b0 ⇒ b1) ->
   (p0 ⇒ p1) ->
   (* ---------- *)
-  (tJ t0 a0 b0 p0) ⇒ (tJ t1 a1 b1 p1)
-| P_JRefl t0 a b t1 :
+  (tJ A0 t0 a0 b0 p0) ⇒ (tJ A1 t1 a1 b1 p1)
+| P_JRefl A t0 a b t1 :
   (t0 ⇒ t1) ->
   (* ---------- *)
-  (tJ t0 a b tRefl) ⇒ t1
+  (tJ A t0 a b tRefl) ⇒ t1
 where "A ⇒ B" := (Par A B).
 
 #[export]Hint Constructors Par : par.
@@ -163,11 +164,6 @@ Lemma Coherent_renaming a b (ξ : fin -> fin) :
   Coherent a⟨ξ⟩ b⟨ξ⟩.
 Proof. hauto lq:on rew:off use:Pars_renaming. Qed.
 
-Local Lemma Par_morphing_lift (ξ0 ξ1 : fin -> tm)
-  (h : forall i, (ξ0 i ⇒ ξ1 i)) :
-  forall i, (up_tm_tm ξ0 i ⇒ up_tm_tm ξ1 i).
-Proof. case => [|i]; first by constructor. asimpl. by apply Par_renaming. Qed.
-
 (* ------------------------------------------------------------ *)
 
 (* Now we want to show all of the ways that these relations are closed 
@@ -183,6 +179,25 @@ Infix "⇒ς*" := (rtc Par_m) (at level 70, right associativity).
 Definition Coherent_m σ0 σ1 :=
   exists σ, (σ0 ⇒ς* σ) /\ (σ1 ⇒ς* σ).
 
+
+Local Fixpoint up_tm_tm_n n ξ :=
+  if n is S n then up_tm_tm_n n (up_tm_tm ξ) else ξ.
+
+Local Lemma Par_morphing_lift_n n (ξ0 ξ1 : fin -> tm)
+  (h : forall i, (ξ0 i ⇒ ξ1 i)) :
+  forall i, (up_tm_tm_n n ξ0 i ⇒ up_tm_tm_n n ξ1 i).
+Proof.
+  elim : n ξ0 ξ1 h =>//.
+  move => n ih ξ0 ξ1 h=>//= i.
+  apply : ih. move => [|i0]//=.
+  by apply Par_refl.
+  by apply Par_renaming.
+Qed.
+
+Local Lemma Par_morphing_lift (ξ0 ξ1 : fin -> tm)
+  (h : forall i, (ξ0 i ⇒ ξ1 i)) :
+  forall i, (up_tm_tm ξ0 i ⇒ up_tm_tm ξ1 i).
+Proof. by apply (Par_morphing_lift_n 1). Qed.
 (* Morphing lemmas *)
 
 Lemma Par_morphing a b (σ0 σ1 : fin -> tm)
@@ -199,7 +214,7 @@ Proof.
     apply P_AppAbs' with (a0 := a0 [up_tm_tm σ]) (b1 := b1 [σ]).
     by asimpl. hauto l:on unfold:Par_m use:Par_renaming inv:nat. eauto.
   - qauto db:par use:Par_morphing_lift.
-  - hauto lq:on db:par use:Par_morphing_lift.
+  - qauto db:par use:(Par_morphing_lift_n 2).
 Qed.
 
 
@@ -403,9 +418,9 @@ Lemma P_IfFalse_star A a b c :
     hauto lq:on ctrs:Par use:Par_refl.
 Qed.
 
-Lemma P_JRefl_star t a b p :
+Lemma P_JRefl_star A t a b p :
   (p ⇒* tRefl)  ->
-  ((tJ t a b p) ⇒* t).
+  ((tJ A t a b p) ⇒* t).
 Proof.
   move E : tRefl => v h.
   move : E.
@@ -449,8 +464,8 @@ Function tstar (a : tm) :=
   | tBool => tBool
   | tRefl => tRefl
   | tEq a b A => tEq (tstar a) (tstar b) (tstar A)
-  | tJ t a b tRefl => tstar t
-  | tJ t a b p => tJ (tstar t) (tstar a) (tstar b) (tstar p)
+  | tJ A t a b tRefl => tstar t
+  | tJ A t a b p => tJ (tstar A) (tstar t) (tstar a) (tstar b) (tstar p)
   end.
 
 Lemma Par_triangle a : forall b, (a ⇒ b) -> (b ⇒ tstar a).
